coq/ZF/Meta/Decl/Axiom/NonEmptyUniverse.v
@@ -1,0 +1,24 @@
+Require Import Coq.Lists.List.
+Require Import Coq.Strings.String.
+
+Require Import ZF.Meta.Env.
+Require Import ZF.Meta.Syntax.
+Require Import ZF.Meta.Term.Decl.
+Require Import ZF.Meta.Ty.
+
+Import ListNotations.
+
+(* exists x, True                                                               *)
+Definition NonEmptyUniverse : DeclT :=
+  {| paraT := []
+  ;  resT  := TyProp
+  ;  bodyT := Ex VarTySet Top
+  |}.
+
+Definition imports : Env := Env.empty.
+
+Definition exports : Env := Env.fromListT
+  [ ("NonEmptyUniverse"%string, NonEmptyUniverse)
+  ].
+
+Definition env : Env := Env.union imports exports.
